theories/iris/logrel/iris_fundamental_drop.v
@@ -42,7 +42,7 @@ Section fundamental.
     iApply (wp_wand _ _ _ (λne vs, interp_val [] vs ∗ ↪[frame] f )%I with "[Hf]").
     { iApply (wp_drop with "Hf"). iRight. iExists []. iNext. iSplit;done. }
     iIntros (v) "[$ Hf]".
-    iExists _;iFrame.
+    iExists _,_;iFrame.
   Qed.
 
 End fundamental.
