theories/iris/logrel/iris_fundamental_segfree.v
@@ -45,7 +45,7 @@ Section fundamental.
     rewrite fixpoint_interp_value_handle_eq.
      iDestruct "Hv" as (h) "(-> & [%Hval | (%γ & %base' & %bound' & #Hw & %Hbase & %Hbound & #Hinv)])".
     { iApply (wp_wand with "[Hf]").
-        - iApply (wp_segfree_failure_1 with "[$Hf]"). 
+        - iApply (wp_segfree_failure1 with "[$Hf]"). 
           + by right.
           + by instantiate (1 := λ x, ⌜ x = trapV ⌝%I).
         - iIntros (v) "[-> Hf]".
@@ -56,7 +56,7 @@ Section fundamental.
 
     destruct (valid h) eqn:Hvalid.
     2: { iApply (wp_wand with "[Hf]").
-        - iApply (wp_segfree_failure_1 with "[$Hf]"). 
+        - iApply (wp_segfree_failure1 with "[$Hf]"). 
           + by right.
           + by instantiate (1 := λ x, ⌜ x = trapV ⌝%I).
         - iIntros (v) "[-> Hf]".
@@ -65,7 +65,7 @@ Section fundamental.
 
     destruct (offset h =? 0)%N eqn:Hoff.
     2:{ apply N.eqb_neq in Hoff. iApply (wp_wand with "[Hf]").
-      - iApply (wp_segfree_failure_1 with "[$Hf]"). 
+      - iApply (wp_segfree_failure1 with "[$Hf]"). 
         + by left.
         + by instantiate (1 := λ x, ⌜ x = trapV ⌝%I).
       - iIntros (v) "[-> Hf]".
@@ -77,148 +77,70 @@ Section fundamental.
     
     iDestruct "Hfv" as "[(%fall & Hbl & Htoks) Hfv]".
     iDestruct (gamma_agree with "Hw Hbl") as "%Hγ".
-    rewrite - (insert_delete _ _ _ Hγ).
-    iDestruct (big_sepM_insert with "Htoks") as "[(%Hx & Ha & Hown) Htoks]";
-      first by rewrite lookup_delete.
-    iApply fupd_wp. Check ghost_map_delete.  Search (ghost_map_auth _ _ (delete _ _)).
-    unfold gamma_id_white.
-    Search (_ ↪[_]□ _ -∗ _ ↪[_] _)%I.
-    iMod (ghost_map_delete with "Hbl [Hw]").
-    { unfold gamma_id_white. iExact "Hw".
-    destruct (base' =? base h)%N eqn:Hnbase.
-    2:{ apply N.eqb_neq in Hnbase. iApply (wp_wand with "[Hf Ha]").
-        - iApply (wp_segfree_failure_2 with "[$Hf $Ha]") => //; try by left.
+(*    iDestruct (big_sepM_lookup_acc _ _ _ _ Hγ with "Htoks") as "[(%y & %Hy & Halloc & Htok) Htoks]". *)
+    rewrite - (insert_delete _ _ _ Hγ). 
+    
+    iDestruct (big_sepM_insert with "Htoks") as "[(%y & %Hy & Halloc & Htok) Htoks]";
+      first by rewrite lookup_delete. 
+    destruct y as [[base0 bound0]|]; first iDestruct "Htok" as "(-> & -> & Htok)".
+    2:{ iApply (wp_wand with "[Hf Halloc]").
+        - iApply (wp_segfree_failure3 with "[$Hf $Halloc]").
+          iIntros "!> Ha".
+          instantiate (1 := λ x, (⌜ x = trapV ⌝ ∗ _)%I).
+          iSplit; last iExact "Ha". done.
+        - iIntros (v) "[[-> Ha] Hf]".
+          iSplitR; first by do 2 iLeft.
+          iExists _,_.
+          iFrame. iExists _. iFrame "Hbl".
+          iApply big_sepM_insert; first by rewrite lookup_delete.
+          iFrame. iExists None. iFrame. done. } 
+    
+    
+    destruct (base0 =? base h)%N eqn:Hnbase.
+    2:{ apply N.eqb_neq in Hnbase. iApply (wp_wand with "[Hf Halloc]").
+        - iApply (wp_segfree_failure2 with "[$Hf $Halloc]") => //; try by left.
           iNext. iIntros "Ha". instantiate (1 := λ x, (⌜ x = trapV ⌝ ∗ _)%I).
           iSplit; first done. iExact "Ha".
         - iIntros (v) "[[-> Ha] Hf]".
           iSplitR; first by do 2 iLeft.
           iExists _, _. iFrame.
-          iExists _. iFrame. admit.  (*rewrite insert_delete => //. 
-          iDestruct (big_sepM_insert. iApply "Htoks". iFrame. done. *)
+          iExists _. iFrame "Hbl". iApply big_sepM_insert; first by rewrite lookup_delete.
+          iFrame. 
+          iExists _. iFrame. done.
     }
-(*    destruct (n0 =? bound h)%N eqn:Hnbound.
-    2:{ apply N.eqb_neq in Hnbound. iApply (wp_wand with "[Hf Ha]").
-        - iApply (wp_segfree_failure_2 with "[$Hf $Ha]") => //; try by right.
-          iNext. iIntros "Ha". instantiate (1 := λ x, (⌜ x = trapV ⌝ ∗ _)%I).
-          iSplit; first done. iExact "Ha".
-        - iIntros (v) "[[-> Ha] Hf]".
-          iSplitR; first by do 2 iLeft.
-          iExists _, _. iFrame.
-          iExists _. iFrame. iApply "Htoks". iExists _. iFrame. done.
-    } *)
+
     iSimpl.
     apply N.eqb_eq in Hnbase as ->.
-(*    apply N.eqb_eq in Hnbound as ->. *)
     iApply fupd_wp. 
-    iMod (cinv_cancel with "Hinv Hown") as "(%tbs & >%Htbs & >Hss & #Hhandles)"; first solve_ndisj.
-      iDestruct (wss_select (N.to_nat (base h)) (N.to_nat bound') (N.to_nat (handle_addr h)) (N.to_nat bound') tbs with "[Hss]") 
+    iMod (cinv_cancel with "Hinv Htok") as "(%tbs & >%Htbs & >Hss & #Hhandles)"; first solve_ndisj.
+    iDestruct (wss_select (N.to_nat (base h)) (N.to_nat bound0) (N.to_nat (handle_addr h)) (N.to_nat bound0) tbs with "[Hss]") 
         as "(%Htbs' & Hss & Hreconstitute)";
         try rewrite N2Nat.id;
         try done;
         try by subst; unfold handle_addr; lia.
-      unfold handle_addr. rewrite Hoff N.add_0_r.
-      unfold handle_addr in Htbs'. rewrite Hoff N.add_0_r in Htbs'. 
+    unfold handle_addr. rewrite Hoff N.add_0_r.
+    unfold handle_addr in Htbs'. rewrite Hoff N.add_0_r in Htbs'. 
     iModIntro.
-    iApply (wp_wand with "[Hf Ha Hss]").
-    { iApply (wp_wand with "[Hf Ha Hss]").
-      - iApply (wp_segfree with "[$Hf $Hss $Ha]") => //.
-        by instantiate (1 := λ x, ⌜ x = immV [] ⌝%I).
-      - iIntros (v) "[-> Hf]". instantiate (1 := λ x, (⌜ x = immV [] ⌝ ∗ ↪[frame] f)%I).
-        by iFrame. }
-    iIntros (v) "[-> Hf]".
-    iSplitR.
-    - iLeft; iRight. iExists _. iSplit => //. 
-    - iExists _,_. iFrame. iExists _. iFrame "Htoks".
-      Search "ghost_map_del".
-      admit.
-      
-    
-  Admitted. 
-(*    unfold semantic_typing, interp_expression.
-    iIntros (i all lh hl).
-    iIntros "#Hi [%Hlh_base [%Hlh_len [%Hlh_valid #Hcont]]]" (f vs) "[Hf Hfv] #Hv".
-    iDestruct "Hv" as "[-> | Hv]".
-    { take_drop_app_rewrite_twice 0 1.
-      iApply (wp_wand _ _ _ (λ vs, ⌜vs = trapV⌝ ∗  ↪[frame]f)%I with "[Hf]").
-      { iApply (wp_trap with "[] [$]");auto. }
-      iIntros (v0) "[? ?]". iFrame. iExists _. iFrame "∗ #". }
-    iDestruct "Hv" as (ws ->) "Hv".
-    iDestruct (big_sepL2_length with "Hv") as %Hlen.
-    destruct ws as [|w ws];[done|destruct ws;[|done]].
-    iSimpl in "Hv". iDestruct "Hv" as "[Hv _]".
-    rewrite fixpoint_interp_value_handle_eq.
-    iDestruct "Hv" as (h γ base' bound') "(-> & #Hw & %Hbase & %Hbound & #Hinv)".
-
-    iSimpl.
-
-
-
-    destruct (valid h) eqn:Hvalid.
-    2:{ iApply (wp_wand with "[Hf]").
-        - iApply (wp_segload_failure with "[$Hf]").
-          + by left.
-          + by instantiate (1 := λ x, ⌜ x = trapV ⌝%I).
-        - iIntros (v) "[-> Hf]".
-          iSplitR; first by do 2 iLeft.
-          iExists _. iFrame. } 
-
-    destruct (bound h <? offset h + N.of_nat (t_length t))%N eqn:Hbounds.
-    { apply N.ltb_lt in Hbounds.
-      iApply (wp_wand with "[Hf]").
-      - iApply (wp_segload_failure with "[$Hf]").
-        + by right; left; lia.
-        + by instantiate (1 := λ x, ⌜ x = trapV ⌝%I).
-      - iIntros (v) "[-> Hf]".
-          iSplitR; first by do 2 iLeft.
-          iExists _. iFrame. } 
-    apply N.ltb_ge in Hbounds.
-
-    iDestruct "Hfv" as "[Halloc Hfv]".
-    iDestruct "Halloc" as (γmap) "[Hbl Htok]".
-    iApply fupd_wp. 
-    iDestruct "Hfv" as (locs Hlocs) "[#Hlocs Hown]".
-    iDestruct (gamma_agree with "Hw Hbl") as "%Hid".
-    iDestruct (big_sepM_lookup_acc _ _ _ _ Hid with "Htok") as "[(%x & %Hx & Halloc & Htok) Htoks]".
-    iMod (cinv_acc with "Hinv Htok") as "(Hss & Hwon & Hcls)"; first solve_ndisj.
-    iDestruct "Hss" as (tbs) "(>%Htbs & >Hss & Hhandles)".
-    iDestruct (wss_select base' bound' (handle_addr h) (N.of_nat (t_length t)) tbs with "Hss")
-      as "(%tbs' & %Htbs' & Hss & Hreconstitute)"; try by subst; unfold handle_addr; lia.
-    assert (length tbs' = t_length t) as Htbs''; first lia. 
-
-    destruct t eqn:Ht.
-
-    - (* Segload T_i32 *)
-      iApply (wp_wand _ _ _ (λ vs, (⌜ vs = immV _ ⌝ ∗ _) ∗ _)%I with "[Hf Halloc Hss]"). 
-      + iApply (wp_segload_deserialize with "[$Hf $Halloc $Hss]") => //.
-      + iIntro (v) "(-> & Halloc & Hss)". iMod ("Hcls" with "[Hss Hhandles]"). iIntros (v).
-    
-    destruct (N_lt_dec (mem_length ms) ((Wasm_int.N_of_uint i32m z) + off + (N.of_nat (t_length t))))%N.
-      { iApply wp_fupd.
-        iApply (wp_wand _ _ _ (λ vs, (⌜vs = trapV⌝ ∗ _) ∗ _)%I with "[Hsize Hf]").
-        { by iApply (wp_load_failure with "[$Hf $Hsize]");[by rewrite Hlocs /=|by apply N.lt_gt|]. }
-        iIntros (v) "[[-> Hsize] Hf]".
-        iMod ("Hcls" with "[$Hown Hsize Hmem]") as "Hown".
-        { iNext. iExists _. iFrame. }
-        iModIntro.
-        iSplitR;[by iLeft; iLeft|iExists _;iFrame].
-        iExists _. eauto. 
-      }
-      { iDestruct (mem_extract _ (Wasm_int.N_of_uint i32m z + off) (t_length t) with "Hmem") as (bv) "[Ha [Hmem %Hlenbv]]";[destruct t;simpl;try lia; try apply hsnz|lia|].
-        iApply wp_fupd.
-        iApply (wp_wand _ _ _ (λ vs, (⌜vs = immV _⌝ ∗ _) ∗ _)%I with "[Ha Hf]").
-        { iApply (wp_load_deserialize with "[$Hf $Ha]");eauto;by rewrite Hlocs /=. }
-        iIntros (v) "[[-> Ha] Hf]".
-        iDestruct ("Hmem" with "Ha") as "Hmem".
-        iMod ("Hcls" with "[$Hown Hsize Hmem]") as "Hown".
-        { iNext. iExists _. iFrame. }
-        iModIntro.
-        iSplitR;[iLeft; iRight|iExists _;iFrame;iExists _;eauto].
-        iExists _. iSplit;[eauto|]. iSimpl.
-        iSplit =>//. unfold interp_value.
-        destruct t;iSimpl;eauto.
-      }
-
-    }
-  Qed. *)
+    iApply (wp_wand with "[Hf Halloc Hss]").
+    - iApply (wp_segfree with "[$Hf $Hss $Halloc]") => //.
+      instantiate (1 := λ x, (⌜ x = immV [] ⌝ ∗ _)%I).
+      iIntros "!> Ha". iSplit; last iExact "Ha". done.
+    - iIntros (v) "[[-> Ha] Hf]".
+      iSplitR.
+      + iLeft; iRight. iExists _. iSplit => //. 
+      + iExists _,({| allocated := <[ id h := None ]> (allocated all); next_free := next_free all |}). iFrame.
+        iExists _. iFrame.
+        iApply big_sepM_insert; first by rewrite lookup_delete.
+        iSplitL "Ha".
+        * iExists None. iFrame. by rewrite lookup_insert.
+        * iApply (big_sepM_impl with "[Htoks]"); first done.
+          iIntros "!>" (k [[γ0 base] bound]) "%Hx (%y & %Hy' & H)".
+          iExists y. iFrame. iPureIntro.
+          simpl. destruct (N.eqb k (id h)) eqn:Hkid.
+          -- apply N.eqb_eq in Hkid as ->.
+             by rewrite lookup_delete in Hx.
+          -- apply N.eqb_neq in Hkid.
+             rewrite lookup_insert_ne => //.
+  Qed. 
 
 End fundamental.
